update

Runwai/Gadget/Func.lean
@@ -2,14 +2,17 @@ import Runwai.Typing
 import Runwai.Gadget.Utils
 import Runwai.Gadget.EnvLemmas
 import Runwai.Gadget.EvalLemmas
+import Runwai.Gadget.TypingLemmas
+import Runwai.Gadget.FieldLemmas
 
 open Ast
 
-abbrev iszero_func := (Ast.Expr.lam "x" (Ast.Ty.refin Ast.Ty.field Ast.constTruePred)
-      (Ast.Expr.lam "y" (Ast.Ty.refin Ast.Ty.field Ast.constTruePred)
-        (Ast.Expr.lam "inv" (Ast.Ty.refin Ast.Ty.field Ast.constTruePred)
-          ((Ast.Expr.letIn "u₁" (.assertE (.var "y") (.fieldExpr (.fieldExpr (.fieldExpr (.constF 0) .sub (.var "x")) .mul (.var "inv")) (.add) (.constF 1)))
-            (Ast.Expr.letIn "u₂" (.assertE (.fieldExpr (.var "x") .mul (.var "y")) (.constF 0)) (.var "u₂")))))))
+abbrev iszero_func: Ast.Expr :=
+  (.lam "x" (Ast.Ty.refin Ast.Ty.field Ast.constTruePred)
+  (.lam "y" (Ast.Ty.refin Ast.Ty.field Ast.constTruePred)
+  (.lam "inv" (Ast.Ty.refin Ast.Ty.field Ast.constTruePred)
+    (.letIn "u₁" (.assertE (.var "y") (.fieldExpr (.fieldExpr (.fieldExpr (.constF 0) .sub (.var "x")) .mul (.var "inv")) (.add) (.constF 1)))
+    (.letIn "u₂" (.assertE (.fieldExpr (.var "x") .mul (.var "y")) (.constF 0)) (.var "u₂"))))))
 
 lemma isZero_eval_eq_branch_semantics {x y inv: Expr} {σ: Env.ValEnv} {Δ: Env.ChipEnv}
   (h₁ : Eval.EvalProp σ Δ (exprEq y ((((Expr.constF 0).fieldExpr FieldOp.sub x).fieldExpr FieldOp.mul inv).fieldExpr
@@ -121,10 +124,10 @@ lemma isZero_typing_soundness (Δ: Env.ChipEnv) (Η: Env.UsedNames) (Γ: Env.TyE
 
 lemma iszero_func_typing_soundness (Δ: Env.ChipEnv) (Η: Env.UsedNames) (Γ: Env.TyEnv) :
   @Ty.TypeJudgment Δ Γ Η iszero_func
-    (Ast.Ty.func "x" (Ast.Ty.refin Ast.Ty.field Ast.constTruePred)
-      (Ast.Ty.func "y" (Ast.Ty.refin Ast.Ty.field Ast.constTruePred)
-        (Ast.Ty.func "inv" (Ast.Ty.refin Ast.Ty.field Ast.constTruePred)
-          (Ty.refin Ast.Ty.unit (Ast.Predicate.ind (exprEq (.var "y") (.branch (.binRel (.var "x") (.eq) (.constF 0)) (.constF 1) (.constF 0)))))))) := by {
+    (Ty.func "x" (Ast.Ty.refin Ast.Ty.field Ast.constTruePred)
+    (Ty.func "y" (Ast.Ty.refin Ast.Ty.field Ast.constTruePred)
+    (Ty.func "inv" (Ast.Ty.refin Ast.Ty.field Ast.constTruePred)
+      (Ty.refin Ast.Ty.unit (Ast.Predicate.ind (exprEq (.var "y") (.branch (.binRel (.var "x") (.eq) (.constF 0)) (.constF 1) (.constF 0)))))))) := by {
       repeat
         apply Ty.TypeJudgment.TE_Abs
         apply lookup_update_self
@@ -141,3 +144,418 @@ lemma iszero_func_typing_soundness (Δ: Env.ChipEnv) (Η: Env.UsedNames) (Γ: En
       apply lookup_update_self
       repeat simp
     }
+
+abbrev koalabear_word_range_checker_func: Ast.Expr :=
+  (.lam "value_0" (Ast.Ty.refin Ast.Ty.field (Ast.Predicate.ind ((Ast.Expr.var "value_0").toZ.binRel Ast.RelOp.lt (Ast.Expr.constZ 256))))
+  (.lam "value_1" (Ast.Ty.refin Ast.Ty.field (Ast.Predicate.ind ((Ast.Expr.var "value_1").toZ.binRel Ast.RelOp.lt (Ast.Expr.constZ 256))))
+  (.lam "value_2" (Ast.Ty.refin Ast.Ty.field (Ast.Predicate.ind ((Ast.Expr.var "value_2").toZ.binRel Ast.RelOp.lt (Ast.Expr.constZ 256))))
+  (.lam "value_3" (Ast.Ty.refin Ast.Ty.field (Ast.Predicate.ind ((Ast.Expr.var "value_3").toZ.binRel Ast.RelOp.lt (Ast.Expr.constZ 256))))
+  (.lam "most_sig_byte_decomp_0" (Ast.Ty.refin Ast.Ty.field Ast.constTruePred)
+  (.lam "most_sig_byte_decomp_1" (Ast.Ty.refin Ast.Ty.field Ast.constTruePred)
+  (.lam "most_sig_byte_decomp_2" (Ast.Ty.refin Ast.Ty.field Ast.constTruePred)
+  (.lam "most_sig_byte_decomp_3" (Ast.Ty.refin Ast.Ty.field Ast.constTruePred)
+  (.lam "most_sig_byte_decomp_4" (Ast.Ty.refin Ast.Ty.field Ast.constTruePred)
+  (.lam "most_sig_byte_decomp_5" (Ast.Ty.refin Ast.Ty.field Ast.constTruePred)
+  (.lam "most_sig_byte_decomp_6" (Ast.Ty.refin Ast.Ty.field Ast.constTruePred)
+  (.lam "most_sig_byte_decomp_7" (Ast.Ty.refin Ast.Ty.field Ast.constTruePred)
+  (.lam "and_most_sig_byte_decomp_0_to_2" (Ast.Ty.refin Ast.Ty.field Ast.constTruePred)
+  (.lam "and_most_sig_byte_decomp_0_to_3" (Ast.Ty.refin Ast.Ty.field Ast.constTruePred)
+  (.lam "and_most_sig_byte_decomp_0_to_4" (Ast.Ty.refin Ast.Ty.field Ast.constTruePred)
+  (.lam "and_most_sig_byte_decomp_0_to_5" (Ast.Ty.refin Ast.Ty.field Ast.constTruePred)
+  (.lam "and_most_sig_byte_decomp_0_to_6" (Ast.Ty.refin Ast.Ty.field Ast.constTruePred)
+  (.lam "and_most_sig_byte_decomp_0_to_7" (Ast.Ty.refin Ast.Ty.field Ast.constTruePred)
+    (.letIn "b₀" (.assertE (.fieldExpr (.var "most_sig_byte_decomp_0") .mul (.fieldExpr (.var "most_sig_byte_decomp_0") .sub (.constF 1))) (.constF 0))
+    (.letIn "b₁" (.assertE (.fieldExpr (.var "most_sig_byte_decomp_1") .mul (.fieldExpr (.var "most_sig_byte_decomp_1") .sub (.constF 1))) (.constF 0))
+    (.letIn "b₂" (.assertE (.fieldExpr (.var "most_sig_byte_decomp_2") .mul (.fieldExpr (.var "most_sig_byte_decomp_2") .sub (.constF 1))) (.constF 0))
+    (.letIn "b₃" (.assertE (.fieldExpr (.var "most_sig_byte_decomp_3") .mul (.fieldExpr (.var "most_sig_byte_decomp_3") .sub (.constF 1))) (.constF 0))
+    (.letIn "b₄" (.assertE (.fieldExpr (.var "most_sig_byte_decomp_4") .mul (.fieldExpr (.var "most_sig_byte_decomp_4") .sub (.constF 1))) (.constF 0))
+    (.letIn "b₅" (.assertE (.fieldExpr (.var "most_sig_byte_decomp_5") .mul (.fieldExpr (.var "most_sig_byte_decomp_5") .sub (.constF 1))) (.constF 0))
+    (.letIn "b₆" (.assertE (.fieldExpr (.var "most_sig_byte_decomp_6") .mul (.fieldExpr (.var "most_sig_byte_decomp_6") .sub (.constF 1))) (.constF 0))
+    (.letIn "b₇" (.assertE (.fieldExpr (.var "most_sig_byte_decomp_7") .mul (.fieldExpr (.var "most_sig_byte_decomp_7") .sub (.constF 1))) (.constF 0))
+    (.letIn "u₁"
+      (.assertE (bits_to_byte_expr "most_sig_byte_decomp_0" "most_sig_byte_decomp_1" "most_sig_byte_decomp_2" "most_sig_byte_decomp_3"
+                                  "most_sig_byte_decomp_4" "most_sig_byte_decomp_5" "most_sig_byte_decomp_6" "most_sig_byte_decomp_7")
+        (.var "value_3")
+      )
+      (.letIn "u₂" (.assertE (.var "most_sig_byte_decomp_7") (.constF 0))
+      (.letIn "u₃" (.assertE (.var "and_most_sig_byte_decomp_0_to_2") (.fieldExpr (.var "most_sig_byte_decomp_0") .mul (.var "most_sig_byte_decomp_1")))
+      (.letIn "u₄" (.assertE (.var "and_most_sig_byte_decomp_0_to_3") (.fieldExpr (.var "and_most_sig_byte_decomp_0_to_2") .mul (.var "most_sig_byte_decomp_2")))
+      (.letIn "u₅" (.assertE (.var "and_most_sig_byte_decomp_0_to_4") (.fieldExpr (.var "and_most_sig_byte_decomp_0_to_3") .mul (.var "most_sig_byte_decomp_3")))
+      (.letIn "u₆" (.assertE (.var "and_most_sig_byte_decomp_0_to_5") (.fieldExpr (.var "and_most_sig_byte_decomp_0_to_4") .mul (.var "most_sig_byte_decomp_4")))
+      (.letIn "u₇" (.assertE (.var "and_most_sig_byte_decomp_0_to_6") (.fieldExpr (.var "and_most_sig_byte_decomp_0_to_5") .mul (.var "most_sig_byte_decomp_5")))
+      (.letIn "u₈" (.assertE (.var "and_most_sig_byte_decomp_0_to_7") (.fieldExpr (.var "and_most_sig_byte_decomp_0_to_6") .mul (.var "most_sig_byte_decomp_6")))
+      (.letIn "u₉" (.assertE (.constF 0) (.fieldExpr (.var "and_most_sig_byte_decomp_0_to_7") .mul (.var "value_0")))
+      (.letIn "u₁₀" (.assertE (.constF 0) (.fieldExpr (.var "and_most_sig_byte_decomp_0_to_7") .mul (.var "value_1")))
+      (.letIn "u₁₁" (.assertE (.constF 0) (.fieldExpr (.var "and_most_sig_byte_decomp_0_to_7") .mul (.var "value_2")))
+        (.var "u₁₁"))))))))))))))))))))))))))))))))))))))
+
+lemma koalabear_word_range_checker_subtype_soundness {Γ Δ}
+  (hb₁: Env.lookupTy Γ "b₀" = some (bit_value_type "most_sig_byte_decomp_0"))
+  (hb₂ : Env.lookupTy Γ "b₁" = some (bit_value_type "most_sig_byte_decomp_1"))
+  (hb₃: Env.lookupTy Γ "b₂" = some (bit_value_type "most_sig_byte_decomp_2"))
+  (hb₄ : Env.lookupTy Γ "b₃" = some (bit_value_type "most_sig_byte_decomp_3"))
+  (hb₅: Env.lookupTy Γ "b₄" = some (bit_value_type "most_sig_byte_decomp_4"))
+  (hb₆ : Env.lookupTy Γ "b₅" = some (bit_value_type "most_sig_byte_decomp_5"))
+  (hb₇: Env.lookupTy Γ "b₆" = some (bit_value_type "most_sig_byte_decomp_6"))
+  (hb₈ : Env.lookupTy Γ "b₇" = some (bit_value_type "most_sig_byte_decomp_7"))
+  (hu₁: Env.lookupTy Γ "u₁" = some (Ast.Ty.unit.refin
+                                  (Ast.Predicate.ind
+                                    (Ast.exprEq
+                                      (bits_to_byte_expr "most_sig_byte_decomp_0" "most_sig_byte_decomp_1" "most_sig_byte_decomp_2" "most_sig_byte_decomp_3"
+                                                        "most_sig_byte_decomp_4" "most_sig_byte_decomp_5" "most_sig_byte_decomp_6" "most_sig_byte_decomp_7")
+                                      (Ast.Expr.var "value_3")))))
+  (hu₂: Env.lookupTy Γ "u₂" = some                               (Ast.Ty.unit.refin
+                                (Ast.Predicate.ind
+                                  (Ast.exprEq (Ast.Expr.var "most_sig_byte_decomp_7") (Ast.Expr.constF 0)))))
+  (hu₃: Env.lookupTy Γ "u₃" = some (eq_mul_refinement "and_most_sig_byte_decomp_0_to_2" "most_sig_byte_decomp_0" "most_sig_byte_decomp_1"))
+  (hu₄: Env.lookupTy Γ "u₄" = some (eq_mul_refinement "and_most_sig_byte_decomp_0_to_3" "and_most_sig_byte_decomp_0_to_2" "most_sig_byte_decomp_2"))
+  (hu₅: Env.lookupTy Γ "u₅" = some (eq_mul_refinement "and_most_sig_byte_decomp_0_to_4" "and_most_sig_byte_decomp_0_to_3" "most_sig_byte_decomp_3"))
+  (hu₆: Env.lookupTy Γ "u₆" = some (eq_mul_refinement "and_most_sig_byte_decomp_0_to_5" "and_most_sig_byte_decomp_0_to_4" "most_sig_byte_decomp_4"))
+  (hu₇: Env.lookupTy Γ "u₇" = some (eq_mul_refinement "and_most_sig_byte_decomp_0_to_6" "and_most_sig_byte_decomp_0_to_5" "most_sig_byte_decomp_5"))
+  (hu₈: Env.lookupTy Γ "u₈" = some (eq_mul_refinement "and_most_sig_byte_decomp_0_to_7" "and_most_sig_byte_decomp_0_to_6" "most_sig_byte_decomp_6"))
+  (hu₉: Env.lookupTy Γ "u₉" = some                           (Ast.Ty.unit.refin
+                  (Ast.Predicate.ind
+                    (Ast.exprEq (Ast.Expr.constF 0)
+                      ((Ast.Expr.var "and_most_sig_byte_decomp_0_to_7").fieldExpr Ast.FieldOp.mul
+                        (Ast.Expr.var "value_0"))))))
+  (hu₁₀: Env.lookupTy Γ "u₁₀" = some                           (Ast.Ty.unit.refin
+                (Ast.Predicate.ind
+                  (Ast.exprEq (Ast.Expr.constF 0)
+                    ((Ast.Expr.var "and_most_sig_byte_decomp_0_to_7").fieldExpr Ast.FieldOp.mul
+                      (Ast.Expr.var "value_1"))))))
+  (hu₁₁: Env.lookupTy Γ "u₁₁" = some                           (Ast.Ty.unit.refin
+                (Ast.Predicate.ind
+                  (Ast.exprEq (Ast.Expr.constF 0)
+                    ((Ast.Expr.var "and_most_sig_byte_decomp_0_to_7").fieldExpr Ast.FieldOp.mul
+                      (Ast.Expr.var "value_2"))))))
+  ( hl₀: Env.lookupTy Γ "value_0" = some (Ast.Ty.refin Ast.Ty.field (Ast.Predicate.ind ((Ast.Expr.var "value_0").toZ.binRel Ast.RelOp.lt (Ast.Expr.constZ 256)))))
+  ( hl₁: Env.lookupTy Γ "value_1" = some (Ast.Ty.refin Ast.Ty.field (Ast.Predicate.ind ((Ast.Expr.var "value_1").toZ.binRel Ast.RelOp.lt (Ast.Expr.constZ 256)))))
+  ( hl₂: Env.lookupTy Γ "value_2" = some (Ast.Ty.refin Ast.Ty.field (Ast.Predicate.ind ((Ast.Expr.var "value_2").toZ.binRel Ast.RelOp.lt (Ast.Expr.constZ 256)))))
+  ( hl₃: Env.lookupTy Γ "value_3" = some (Ast.Ty.refin Ast.Ty.field (Ast.Predicate.ind ((Ast.Expr.var "value_3").toZ.binRel Ast.RelOp.lt (Ast.Expr.constZ 256)))))
+  : @Ty.SubtypeJudgment Δ Γ
+      (Ty.unit.refin (Predicate.ind (exprEq (Expr.constF 0) ((Expr.var "and_most_sig_byte_decomp_0_to_7").fieldExpr FieldOp.mul (Expr.var "value_2")))))
+      (Ast.Ty.refin Ast.Ty.unit (Ast.Predicate.ind
+              (.binRel (.integerExpr (.integerExpr (.integerExpr
+                (.toZ (.var "value_0")) .add (.integerExpr (.toZ (.var "value_1")) .mul (.constZ 256)))
+                                        .add (.integerExpr (.toZ (.var "value_2")) .mul (.constZ (256^2))))
+                                        .add (.integerExpr (.toZ (.var "value_3")) .mul (.constZ (256^3))))
+              .lt (.constZ 2130706433)))) := by {
+    apply Ty.SubtypeJudgment.TSub_Refine
+    apply Ty.SubtypeJudgment.TSub_Refl
+    intro σ v h₁ h₂
+
+    have hb₁' := tyenv_to_eval_expr h₁ hb₁
+    have hb₂' := tyenv_to_eval_expr h₁ hb₂
+    have hb₃' := tyenv_to_eval_expr h₁ hb₃
+    have hb₄' := tyenv_to_eval_expr h₁ hb₄
+    have hb₅' := tyenv_to_eval_expr h₁ hb₅
+    have hb₆' := tyenv_to_eval_expr h₁ hb₆
+    have hb₇' := tyenv_to_eval_expr h₁ hb₇
+    have hb₈' := tyenv_to_eval_expr h₁ hb₈
+    have hu₁' := tyenv_to_eval_expr h₁ hu₁
+    have hu₂' := tyenv_to_eval_expr h₁ hu₂
+    have hu₃' := tyenv_to_eval_expr h₁ hu₃
+    have hu₄' := tyenv_to_eval_expr h₁ hu₄
+    have hu₅' := tyenv_to_eval_expr h₁ hu₅
+    have hu₆' := tyenv_to_eval_expr h₁ hu₆
+    have hu₇' := tyenv_to_eval_expr h₁ hu₇
+    have hu₈' := tyenv_to_eval_expr h₁ hu₈
+    have hu₉' := tyenv_to_eval_expr h₁ hu₉
+    have hu₁₀' := tyenv_to_eval_expr h₁ hu₁₀
+    have hu₁₁' := tyenv_to_eval_expr h₁ hu₁₁
+    have hl₀' := tyenv_to_eval_expr h₁ hl₀
+    have hl₁' := tyenv_to_eval_expr h₁ hl₁
+    have hl₂' := tyenv_to_eval_expr h₁ hl₂
+    have hl₃' := tyenv_to_eval_expr h₁ hl₃
+
+    have hb₁'' := eval_bit_expr_val hb₁'
+    have hb₂'' := eval_bit_expr_val hb₂'
+    have hb₃'' := eval_bit_expr_val hb₃'
+    have hb₄'' := eval_bit_expr_val hb₄'
+    have hb₅'' := eval_bit_expr_val hb₅'
+    have hb₆'' := eval_bit_expr_val hb₆'
+    have hb₇'' := eval_bit_expr_val hb₇'
+    have hb₈'' := eval_bit_expr_val hb₈'
+    have hu₁' := eval_bits_to_byte_expr_val hu₁'
+    have hu₃'' := eval_mul_expr_val hu₃'
+    have hu₄'' := eval_mul_expr_val hu₄'
+    have hu₅'' := eval_mul_expr_val hu₅'
+    have hu₆'' := eval_mul_expr_val hu₆'
+    have hu₇'' := eval_mul_expr_val hu₇'
+    have hu₈'' := eval_mul_expr_val hu₈'
+    have hu₉'' := eval_eq_const_mul_val hu₉'
+    have hu₁₀'' := eval_eq_const_mul_val hu₁₀'
+    have hu₁₁'' := eval_eq_const_mul_val hu₁₁'
+    have hvl₀ := eval_lt_val hl₀'
+    have hvl₁ := eval_lt_val hl₁'
+    have hvl₂ := eval_lt_val hl₂'
+    have hvl₃ := eval_lt_val hl₃'
+
+    cases hu₂'
+    rename_i v₁ u₁ ih₁ ih₂ h_most_sig_byte_decomp_7_is_0
+    cases ih₁
+    cases ih₂
+    unfold Eval.evalRelOp at h_most_sig_byte_decomp_7_is_0
+    cases v₁ <;> simp at h_most_sig_byte_decomp_7_is_0
+    rename_i most_sig_byte_decomp_7 h_most_sig_byte_decomp_7_env
+
+    unfold PropSemantics.predToProp PropSemantics.exprToProp
+    obtain ⟨most_sig_byte_decomp_0, h⟩ := hb₁''
+    obtain ⟨h_most_sig_byte_decomp_0_env, h_most_sig_byte_decomp_0⟩ := h
+    obtain ⟨most_sig_byte_decomp_1, h⟩ := hb₂''
+    obtain ⟨h_most_sig_byte_decomp_1_env, h_most_sig_byte_decomp_1⟩ := h
+    obtain ⟨most_sig_byte_decomp_2, h⟩ := hb₃''
+    obtain ⟨h_most_sig_byte_decomp_2_env, h_most_sig_byte_decomp_2⟩ := h
+    obtain ⟨most_sig_byte_decomp_3, h⟩ := hb₄''
+    obtain ⟨h_most_sig_byte_decomp_3_env, h_most_sig_byte_decomp_3⟩ := h
+    obtain ⟨most_sig_byte_decomp_4, h⟩ := hb₅''
+    obtain ⟨h_most_sig_byte_decomp_4_env, h_most_sig_byte_decomp_4⟩ := h
+    obtain ⟨most_sig_byte_decomp_5, h⟩ := hb₆''
+    obtain ⟨h_most_sig_byte_decomp_5_env, h_most_sig_byte_decomp_5⟩ := h
+    obtain ⟨most_sig_byte_decomp_6, h⟩ := hb₇''
+    obtain ⟨h_most_sig_byte_decomp_6_env, h_most_sig_byte_decomp_6⟩ := h
+    obtain ⟨most_sig_byte_decomp_7', h⟩ := hb₈''
+    obtain ⟨h_most_sig_byte_decomp_7_env', h_most_sig_byte_decomp_7⟩ := h
+    rw[h_most_sig_byte_decomp_7_env] at h_most_sig_byte_decomp_7_env'
+    simp at h_most_sig_byte_decomp_7_env'
+    rw[← h_most_sig_byte_decomp_7_env'] at h_most_sig_byte_decomp_7
+
+    obtain ⟨v₀, v₁, v₂, v₃, v₄, v₅, v₆, v₇, value_3, h⟩ := hu₁'
+    obtain ⟨h₁, h₂, h₃, h₄, h₅, h₆, h₇, h₈, h_value_3_env, h_msb_rec⟩ := h
+    simp at h_most_sig_byte_decomp_0_env h_most_sig_byte_decomp_1_env
+            h_most_sig_byte_decomp_2_env h_most_sig_byte_decomp_3_env
+            h_most_sig_byte_decomp_4_env h_most_sig_byte_decomp_5_env
+            h_most_sig_byte_decomp_6_env h_most_sig_byte_decomp_7_env
+    rw[h_most_sig_byte_decomp_0_env] at h₁
+    rw[h_most_sig_byte_decomp_1_env] at h₂
+    rw[h_most_sig_byte_decomp_2_env] at h₃
+    rw[h_most_sig_byte_decomp_3_env] at h₄
+    rw[h_most_sig_byte_decomp_4_env] at h₅
+    rw[h_most_sig_byte_decomp_5_env] at h₆
+    rw[h_most_sig_byte_decomp_6_env] at h₇
+    rw[h_most_sig_byte_decomp_7_env] at h₈
+    simp at h₁ h₂ h₃ h₄ h₅ h₆ h₇ h₈ h_value_3_env
+    rw[← h₁, ← h₂, ← h₃, ← h₄, ← h₅, ← h₆, ← h₇, ← h₈] at h_msb_rec
+
+    obtain ⟨and_most_sig_byte_decomp_0_to_2, v₂, v₃, h⟩ := hu₃''
+    obtain ⟨h_and_most_sig_byte_decomp_0_to_2_env, h₂, h₃, hamm₁⟩ := h
+    simp at h_and_most_sig_byte_decomp_0_to_2_env h₂ h₃ hamm₁
+    rw[h_most_sig_byte_decomp_0_env] at h₂
+    rw[h_most_sig_byte_decomp_1_env] at h₃
+    simp at h₂ h₃ hamm₁
+    rw[← h₂, ← h₃] at hamm₁
+
+
+    obtain ⟨and_most_sig_byte_decomp_0_to_3, v₂, v₃, h⟩ := hu₄''
+    obtain ⟨h_and_most_sig_byte_decomp_0_to_3_env, h₂, h₃, hamm₂⟩ := h
+    simp at h_and_most_sig_byte_decomp_0_to_3_env h₂ h₃ hamm₂
+    rw[h_and_most_sig_byte_decomp_0_to_2_env] at h₂
+    rw[h_most_sig_byte_decomp_2_env] at h₃
+    simp at h₂ h₃ hamm₂
+    rw[← h₂, ← h₃] at hamm₂
+
+    obtain ⟨and_most_sig_byte_decomp_0_to_4, v₂, v₃, h⟩ := hu₅''
+    obtain ⟨h_and_most_sig_byte_decomp_0_to_4_env, h₂, h₃, hamm₃⟩ := h
+    simp at h_and_most_sig_byte_decomp_0_to_4_env h₂ h₃ hamm₃
+    rw[h_and_most_sig_byte_decomp_0_to_3_env] at h₂
+    rw[h_most_sig_byte_decomp_3_env] at h₃
+    simp at h₂ h₃ hamm₃
+    rw[← h₂, ← h₃] at hamm₃
+
+    obtain ⟨and_most_sig_byte_decomp_0_to_5, v₂, v₃, h⟩ := hu₆''
+    obtain ⟨h_and_most_sig_byte_decomp_0_to_5_env, h₂, h₃, hamm₄⟩ := h
+    simp at h_and_most_sig_byte_decomp_0_to_5_env h₂ h₃ hamm₄
+    rw[h_and_most_sig_byte_decomp_0_to_4_env] at h₂
+    rw[h_most_sig_byte_decomp_4_env] at h₃
+    simp at h₂ h₃ hamm₄
+    rw[← h₂, ← h₃] at hamm₄
+
+    obtain ⟨and_most_sig_byte_decomp_0_to_6, v₂, v₃, h⟩ := hu₇''
+    obtain ⟨h_and_most_sig_byte_decomp_0_to_6_env, h₂, h₃, hamm₅⟩ := h
+    simp at h_and_most_sig_byte_decomp_0_to_6_env h₂ h₃ hamm₅
+    rw[h_and_most_sig_byte_decomp_0_to_5_env] at h₂
+    rw[h_most_sig_byte_decomp_5_env] at h₃
+    simp at h₂ h₃ hamm₅
+    rw[← h₂, ← h₃] at hamm₅
+
+    obtain ⟨and_most_sig_byte_decomp_0_to_7, v₂, v₃, h⟩ := hu₈''
+    obtain ⟨h_and_most_sig_byte_decomp_0_to_7_env, h₂, h₃, hamm₆⟩ := h
+    simp at h_and_most_sig_byte_decomp_0_to_7_env h₂ h₃ hamm₆
+    rw[h_and_most_sig_byte_decomp_0_to_6_env] at h₂
+    rw[h_most_sig_byte_decomp_6_env] at h₃
+    simp at h₂ h₃ hamm₆
+    rw[← h₂, ← h₃] at hamm₆
+
+    obtain ⟨v₁, value_0, h⟩ := hu₉''
+    obtain ⟨h₁, h_value_0_env, hav₀⟩ := h
+    simp at h₁ h_value_0_env hav₀
+    rw[h_and_most_sig_byte_decomp_0_to_7_env] at h₁
+    simp at h₁
+    rw[← h₁] at hav₀
+
+
+    obtain ⟨v₁, value_1, h⟩ := hu₁₀''
+    obtain ⟨h₁, h_value_1_env, hav₁⟩ := h
+    simp at h₁ h_value_1_env hav₁
+    rw[h_and_most_sig_byte_decomp_0_to_7_env] at h₁
+    simp at h₁
+    rw[← h₁] at hav₁
+
+    obtain ⟨v₁, value_2, h⟩ := hu₁₁''
+    obtain ⟨h₁, h_value_2_env, hav₂⟩ := h
+    simp at h₁ h_value_2_env hav₂
+    rw[h_and_most_sig_byte_decomp_0_to_7_env] at h₁
+    simp at h₁
+    rw[← h₁] at hav₂
+
+    obtain ⟨v₁, h₁, hvl₀⟩ := hvl₀
+    simp at h₁
+    rw[h_value_0_env] at h₁
+    simp at h₁
+    rw[← h₁] at hvl₀
+
+    obtain ⟨v₁, h₁, hvl₁⟩ := hvl₁
+    simp at h₁
+    rw[h_value_1_env] at h₁
+    simp at h₁
+    rw[← h₁] at hvl₁
+
+    obtain ⟨v₁, h₁, hvl₂⟩ := hvl₂
+    simp at h₁
+    rw[h_value_2_env] at h₁
+    simp at h₁
+    rw[← h₁] at hvl₂
+
+    obtain ⟨v₁, h₁, hvl₃⟩ := hvl₃
+    simp at h₁
+    rw[h_value_3_env] at h₁
+    simp at h₁
+    rw[← h₁] at hvl₃
+
+    repeat
+      repeat constructor
+      assumption
+    repeat constructor
+    simp
+
+    apply word32_range_under_koalabear
+      (bit_value_mul_zero h_most_sig_byte_decomp_0) (bit_value_mul_zero h_most_sig_byte_decomp_1)
+      (bit_value_mul_zero h_most_sig_byte_decomp_2) (bit_value_mul_zero h_most_sig_byte_decomp_3)
+      (bit_value_mul_zero h_most_sig_byte_decomp_4) (bit_value_mul_zero h_most_sig_byte_decomp_5)
+      (bit_value_mul_zero h_most_sig_byte_decomp_6) (bit_value_mul_zero h_most_sig_byte_decomp_7)
+      h_msb_rec h_most_sig_byte_decomp_7_is_0 hamm₁ hamm₂ hamm₃ hamm₄ hamm₅ hamm₆
+    simp
+    exact hav₀
+    simp
+    exact hav₁
+    simp
+    repeat assumption
+}
+
+lemma koalabear_word_range_checker_func_typing_soundness (Δ: Env.ChipEnv) (Η: Env.UsedNames) (Γ: Env.TyEnv) :
+  @Ty.TypeJudgment Δ Γ Η koalabear_word_range_checker_func
+    (Ast.Ty.func "value_0" (Ast.Ty.refin Ast.Ty.field (Ast.Predicate.ind ((Ast.Expr.var "value_0").toZ.binRel Ast.RelOp.lt (Ast.Expr.constZ 256))))
+    (Ast.Ty.func "value_1" (Ast.Ty.refin Ast.Ty.field (Ast.Predicate.ind ((Ast.Expr.var "value_1").toZ.binRel Ast.RelOp.lt (Ast.Expr.constZ 256))))
+    (Ast.Ty.func "value_2" (Ast.Ty.refin Ast.Ty.field (Ast.Predicate.ind ((Ast.Expr.var "value_2").toZ.binRel Ast.RelOp.lt (Ast.Expr.constZ 256))))
+    (Ast.Ty.func "value_3" (Ast.Ty.refin Ast.Ty.field (Ast.Predicate.ind ((Ast.Expr.var "value_3").toZ.binRel Ast.RelOp.lt (Ast.Expr.constZ 256))))
+    (Ast.Ty.func "most_sig_byte_decomp_0" (Ast.Ty.refin Ast.Ty.field Ast.constTruePred)
+    (Ast.Ty.func "most_sig_byte_decomp_1" (Ast.Ty.refin Ast.Ty.field Ast.constTruePred)
+    (Ast.Ty.func "most_sig_byte_decomp_2" (Ast.Ty.refin Ast.Ty.field Ast.constTruePred)
+    (Ast.Ty.func "most_sig_byte_decomp_3" (Ast.Ty.refin Ast.Ty.field Ast.constTruePred)
+    (Ast.Ty.func "most_sig_byte_decomp_4" (Ast.Ty.refin Ast.Ty.field Ast.constTruePred)
+    (Ast.Ty.func "most_sig_byte_decomp_5" (Ast.Ty.refin Ast.Ty.field Ast.constTruePred)
+    (Ast.Ty.func "most_sig_byte_decomp_6" (Ast.Ty.refin Ast.Ty.field Ast.constTruePred)
+    (Ast.Ty.func "most_sig_byte_decomp_7" (Ast.Ty.refin Ast.Ty.field Ast.constTruePred)
+    (Ast.Ty.func "and_most_sig_byte_decomp_0_to_2" (Ast.Ty.refin Ast.Ty.field Ast.constTruePred)
+    (Ast.Ty.func "and_most_sig_byte_decomp_0_to_3" (Ast.Ty.refin Ast.Ty.field Ast.constTruePred)
+    (Ast.Ty.func "and_most_sig_byte_decomp_0_to_4" (Ast.Ty.refin Ast.Ty.field Ast.constTruePred)
+    (Ast.Ty.func "and_most_sig_byte_decomp_0_to_5" (Ast.Ty.refin Ast.Ty.field Ast.constTruePred)
+    (Ast.Ty.func "and_most_sig_byte_decomp_0_to_6" (Ast.Ty.refin Ast.Ty.field Ast.constTruePred)
+    (Ast.Ty.func "and_most_sig_byte_decomp_0_to_7" (Ast.Ty.refin Ast.Ty.field Ast.constTruePred)
+      (Ast.Ty.refin Ast.Ty.unit (Ast.Predicate.ind
+        (.binRel (.integerExpr (.integerExpr (.integerExpr
+          (.toZ (.var "value_0")) .add (.integerExpr (.toZ (.var "value_1")) .mul (.constZ 256)))
+                                  .add (.integerExpr (.toZ (.var "value_2")) .mul (.constZ (256^2))))
+                                  .add (.integerExpr (.toZ (.var "value_3")) .mul (.constZ (256^3))))
+        .lt (.constZ 2130706433)))))))))))))))))))))) := by {
+  repeat
+    apply Ty.TypeJudgment.TE_Abs
+    apply lookup_update_self
+  repeat
+    apply Ty.TypeJudgment.TE_LetIn;
+    apply lookup_update_self;
+    apply Ty.TypeJudgment.TE_Assert
+    apply Ty.TypeJudgment.TE_BinOpField
+    apply Ty.TypeJudgment.TE_VarEnv
+    apply lookup_update_ne
+    simp
+    apply Ty.TypeJudgment.TE_BinOpField
+    apply Ty.TypeJudgment.TE_VarEnv
+    apply lookup_update_ne
+    simp
+    repeat apply Ty.TypeJudgment.TE_ConstF
+  apply Ty.TypeJudgment.TE_LetIn;
+  apply lookup_update_self;
+  apply Ty.TypeJudgment.TE_Assert
+  repeat apply Ty.TypeJudgment.TE_BinOpField
+  apply Ty.TypeJudgment.TE_VarEnv
+  apply lookup_update_ne
+  simp
+  repeat
+    apply Ty.TypeJudgment.TE_BinOpField
+    apply Ty.TypeJudgment.TE_VarEnv
+    apply lookup_update_ne
+    simp
+    repeat apply Ty.TypeJudgment.TE_ConstF
+  apply Ty.TypeJudgment.TE_VarEnv
+  apply lookup_update_ne
+  simp
+
+  apply Ty.TypeJudgment.TE_LetIn;
+  apply lookup_update_self;
+  apply Ty.TypeJudgment.TE_Assert
+  apply Ty.TypeJudgment.TE_VarEnv
+  apply lookup_update_ne
+  simp
+  apply Ty.TypeJudgment.TE_ConstF
+
+  repeat
+    apply Ty.TypeJudgment.TE_LetIn;
+    apply lookup_update_self;
+    apply Ty.TypeJudgment.TE_Assert
+    apply Ty.TypeJudgment.TE_VarEnv
+    apply lookup_update_ne
+    simp
+    apply Ty.TypeJudgment.TE_BinOpField
+    repeat
+      apply Ty.TypeJudgment.TE_VarEnv
+      apply lookup_update_ne
+      simp
+
+  repeat
+    apply Ty.TypeJudgment.TE_LetIn;
+    apply lookup_update_self;
+    apply Ty.TypeJudgment.TE_Assert
+    apply Ty.TypeJudgment.TE_ConstF
+    apply Ty.TypeJudgment.TE_BinOpField
+    repeat
+      apply Ty.TypeJudgment.TE_VarEnv
+      apply lookup_update_ne
+      simp
+
+  apply Ty.TypeJudgment.TE_SUB
+  apply Ty.TypeJudgment.TE_VarEnv
+  apply lookup_update_self
+  apply koalabear_word_range_checker_subtype_soundness
+  repeat
+    apply lookup_update_ne
+    simp
+  apply lookup_update_self
+  repeat
+    apply lookup_update_ne
+    simp
+}
+
+/-
+koalabear_word_range_checker_func
+-/
